src/Examples/QueryStructure/Messages.v
@@ -1,7 +1,4 @@
-Require Import Coq.Strings.String.
-Require Import Fiat.QueryStructure.Automation.AutoDB
-        Fiat.QueryStructure.Automation.IndexSelection
-        Fiat.QueryStructure.Automation.QSImplementation.
+Require Import Fiat.QueryStructure.Automation.MasterPlan.
 
 Definition MESSAGES := "Messages".
 Definition CONTACTS := "Contacts".
@@ -68,61 +65,12 @@ Definition SharpenedMessages :
   FullySharpened MessagesSpec.
 Proof.
 
-  start_honing_QueryStructure.
-
-  {
-
-    GenerateIndexesForAll
-      ltac:(CombineCase3 matchInclusionIndex matchEqIndex)
-             ltac:(fun attrList =>
-                     make_simple_indexes
-                       attrList
-                       ltac:(CombineCase6 BuildEarlyEqualityIndex
-                                          ltac:(fun _ _ _ _ _ _ => fail))
-                              ltac:(CombineCase5 BuildLastEqualityIndex
-                                                 ltac:(CombineCase5
-                                                         BuildLastInclusionIndex
-                                                         ltac:(fun _ _ _ _ _ => fail)))).
-    - initializer.
-    - insertion ltac:(CombineCase5 InclusionIndexUse EqIndexUse)
-             ltac:(CombineCase10 createEarlyInclusionTerm createEarlyEqualityTerm)
-                    ltac:(CombineCase7 createLastInclusionTerm createLastEqualityTerm)
-                           ltac:(CombineCase7 InclusionIndexUse_dep EqIndexUse_dep)
-                                  ltac:(CombineCase11 createEarlyInclusionTerm_dep createEarlyEqualityTerm_dep)
-                                         ltac:(CombineCase8 createLastInclusionTerm_dep createLastEqualityTerm_dep).
-    - insertion ltac:(CombineCase5 InclusionIndexUse EqIndexUse)
-             ltac:(CombineCase10 createEarlyInclusionTerm createEarlyEqualityTerm)
-                    ltac:(CombineCase7 createLastInclusionTerm createLastEqualityTerm)
-                           ltac:(CombineCase7 InclusionIndexUse_dep EqIndexUse_dep)
-                                  ltac:(CombineCase11 createEarlyInclusionTerm_dep createEarlyEqualityTerm_dep)
-                                         ltac:(CombineCase8 createLastInclusionTerm_dep createLastEqualityTerm_dep).
-    - observer ltac:(CombineCase5 InclusionIndexUse EqIndexUse)
-             ltac:(CombineCase10 createEarlyInclusionTerm createEarlyEqualityTerm)
-                    ltac:(CombineCase7 createLastInclusionTerm createLastEqualityTerm)
-                           ltac:(CombineCase7 InclusionIndexUse_dep EqIndexUse_dep)
-                                  ltac:(CombineCase11 createEarlyInclusionTerm_dep createEarlyEqualityTerm_dep)
-                                         ltac:(CombineCase8 createLastInclusionTerm_dep createLastEqualityTerm_dep).
-    - observer ltac:(CombineCase5 InclusionIndexUse EqIndexUse)
-             ltac:(CombineCase10 createEarlyInclusionTerm createEarlyEqualityTerm)
-                    ltac:(CombineCase7 createLastInclusionTerm createLastEqualityTerm)
-                           ltac:(CombineCase7 InclusionIndexUse_dep EqIndexUse_dep)
-                                  ltac:(CombineCase11 createEarlyInclusionTerm_dep createEarlyEqualityTerm_dep)
-                                         ltac:(CombineCase8 createLastInclusionTerm_dep createLastEqualityTerm_dep).
-    - pose_headings_all.
-      match goal with
-      | |- appcontext[@BuildADT (IndexedQueryStructure ?Schema ?Indexes)] =>
-        FullySharpenQueryStructure Schema Indexes
-      end.
-  }
-
-  { simpl; pose_string_ids; pose_headings_all;
-    pose_search_term; pose_SearchUpdateTerms.
-    BuildQSIndexedBags' BuildEarlyEqualityBag
-                        ltac:(CombineCase5 BuildLastInclusionIndexBag BuildLastEqualityBag).
-  }
-  higher_order_reflexivityT.
+  (* Uncomment this to see the mostly sharpened implementation *)
+  (* partial_master_plan ltac:(CombineIndexTactics InclusionIndexTactics EqIndexTactics). *)
+  master_plan ltac:(CombineIndexTactics InclusionIndexTactics EqIndexTactics).
 
 Time Defined.
-
+(* 1336MB *)
 Time Definition MessagesImpl : ComputationalADT.cADT MessagesSig :=
   Eval simpl in (projT1 SharpenedMessages).
+Print MessagesImpl.
