src/Examples/QueryStructure/Photoalbum.v
@@ -1,7 +1,4 @@
-Require Import Coq.Strings.String.
-Require Import Fiat.QueryStructure.Automation.AutoDB
-        Fiat.QueryStructure.Automation.IndexSelection
-        Fiat.QueryStructure.Automation.QSImplementation.
+Require Import Fiat.QueryStructure.Automation.MasterPlan.
 
 Definition PHOTOS := "Photos".
 Definition EVENTS := "Events".
@@ -67,61 +64,16 @@ Definition SharpenedAlbum :
   FullySharpened AlbumSpec.
 Proof.
 
-  start honing QueryStructure.
-
-  {
-  (* Manually select indexes + data structure. *)
-let attrList := constr:(icons3 (B := fun heading => list (prod string (Attributes (rawSchemaHeading heading)))) (a := Vector.hd (qschemaSchemas AlbumSchema)) [("EqualityIndex", Fin.FS (Fin.FS (@Fin.F1 0))); ("InclusionIndex", Fin.FS (@Fin.F1 1))] (icons3 (a := Vector.hd (Vector.tl (qschemaSchemas AlbumSchema))) [("EqualityIndex", @Fin.F1 1); ("RangeIndex", Fin.FS (@Fin.F1 0))] inil3)) in
-make_simple_indexes attrList
-  ltac:(CombineCase6 BuildEarlyEqualityIndex
-                     ltac:(CombineCase6 BuildEarlyRangeIndex
-                                        ltac:(fun _ _ _ _ _ _ => fail)))
-         ltac:(CombineCase5 BuildLastEqualityIndex
-                            ltac:(CombineCase5
-
-                                    BuildLastInclusionIndex ltac:(CombineCase5 BuildLastRangeIndex
-                                                                               ltac:(fun _ _ _ _ _ => fail)))).
-
-    - initializer.
-    - insertion ltac:(CombineCase5 InclusionIndexUse ltac:(CombineCase5 RangeIndexUse EqIndexUse))
-             ltac:(CombineCase10 createEarlyInclusionTerm ltac:(CombineCase10 createEarlyRangeTerm createEarlyEqualityTerm))
-                    ltac:(CombineCase7 createLastInclusionTerm ltac:(CombineCase7 createLastRangeTerm createLastEqualityTerm))
-                           ltac:(CombineCase7 InclusionIndexUse_dep ltac:(CombineCase7 RangeIndexUse_dep EqIndexUse_dep))
-                                  ltac:(CombineCase11 createEarlyInclusionTerm_dep ltac:(CombineCase11 createEarlyRangeTerm_dep createEarlyEqualityTerm_dep))
-                                         ltac:(CombineCase8 createLastInclusionTerm_dep ltac:(CombineCase8 createLastRangeTerm_dep createLastEqualityTerm_dep)).
-    - insertion ltac:(CombineCase5 InclusionIndexUse ltac:(CombineCase5 RangeIndexUse EqIndexUse))
-             ltac:(CombineCase10 createEarlyInclusionTerm ltac:(CombineCase10 createEarlyRangeTerm createEarlyEqualityTerm))
-                    ltac:(CombineCase7 createLastInclusionTerm ltac:(CombineCase7 createLastRangeTerm createLastEqualityTerm))
-                           ltac:(CombineCase7 InclusionIndexUse_dep ltac:(CombineCase7 RangeIndexUse_dep EqIndexUse_dep))
-                                  ltac:(CombineCase11 createEarlyInclusionTerm_dep ltac:(CombineCase11 createEarlyRangeTerm_dep createEarlyEqualityTerm_dep))
-                                         ltac:(CombineCase8 createLastInclusionTerm_dep ltac:(CombineCase8 createLastRangeTerm_dep createLastEqualityTerm_dep)).
-    - observer ltac:(CombineCase5 InclusionIndexUse ltac:(CombineCase5 RangeIndexUse EqIndexUse))
-             ltac:(CombineCase10 createEarlyInclusionTerm ltac:(CombineCase10 createEarlyRangeTerm createEarlyEqualityTerm))
-                    ltac:(CombineCase7 createLastInclusionTerm ltac:(CombineCase7 createLastRangeTerm createLastEqualityTerm))
-                           ltac:(CombineCase7 InclusionIndexUse_dep ltac:(CombineCase7 RangeIndexUse_dep EqIndexUse_dep))
-                                  ltac:(CombineCase11 createEarlyInclusionTerm_dep ltac:(CombineCase11 createEarlyRangeTerm_dep createEarlyEqualityTerm_dep))
-                                         ltac:(CombineCase8 createLastInclusionTerm_dep ltac:(CombineCase8 createLastRangeTerm_dep createLastEqualityTerm_dep)).
-    - observer ltac:(CombineCase5 InclusionIndexUse ltac:(CombineCase5 RangeIndexUse EqIndexUse))
-             ltac:(CombineCase10 createEarlyInclusionTerm ltac:(CombineCase10 createEarlyRangeTerm createEarlyEqualityTerm))
-                    ltac:(CombineCase7 createLastInclusionTerm ltac:(CombineCase7 createLastRangeTerm createLastEqualityTerm))
-                           ltac:(CombineCase7 InclusionIndexUse_dep ltac:(CombineCase7 RangeIndexUse_dep EqIndexUse_dep))
-                                  ltac:(CombineCase11 createEarlyInclusionTerm_dep ltac:(CombineCase11 createEarlyRangeTerm_dep createEarlyEqualityTerm_dep))
-                                         ltac:(CombineCase8 createLastInclusionTerm_dep ltac:(CombineCase8 createLastRangeTerm_dep createLastEqualityTerm_dep)).
-    - pose_headings_all.
-
-     match goal with
-     | |- appcontext[@BuildADT (IndexedQueryStructure ?Schema ?Indexes)] =>
-       FullySharpenQueryStructure Schema Indexes
-     end.
-     }
-
-  { simpl; pose_string_ids; pose_headings_all;
-    pose_search_term; pose_SearchUpdateTerms.
-
-BuildQSIndexedBags' ltac:(CombineCase6 BuildEarlyRangeTreeBag BuildEarlyEqualityBag)
-                        ltac:(CombineCase5 BuildLastInclusionIndexBag
-                                           ltac:(CombineCase5 BuildLastRangeTreeBag BuildLastEqualityBag)).
-  }
-  higher_order_reflexivityT.
-
+  (* Uncomment this to see the mostly sharpened implementation *)
+  (* partial_master_plan ltac:(CombineIndexTactics InclusionIndexTactics
+          ltac:(CombineIndexTactics RangeIndexTactics EqIndexTactics)).*)
+  master_plan
+    ltac:(CombineIndexTactics InclusionIndexTactics
+          ltac:(CombineIndexTactics RangeIndexTactics EqIndexTactics)).
 Time Defined.
+(*Mem: 1380MB *)
+
+Time Definition AlbumImpl : ComputationalADT.cADT AlbumSig :=
+  Eval simpl in (projT1 SharpenedAlbum).
+(* Mem: 1028MB *)
+Print AlbumImpl.
